src/impl/TLS13.Impl.Server.fst
@@ -1,0 +1,110 @@
+module TLS13.Impl.Server
+
+#lang-pulse
+
+open Pulse.Lib.Pervasives
+open Pulse.Lib.Array.PtsTo
+
+module B = TLS13.Bytes
+module CS = TLS13.Spec.ConnectionState
+module CSL = TLS13.ConnectionState.Lemmas
+module CR = TLS13.Impl.ConnectionState.Repr
+module ST = TLS13.Impl.Server.Types
+module SZ = FStar.SizeT
+module U8 = FStar.UInt8
+
+fn new_server
+  (certificate_chain:array U8.t)
+  (certificate_chain_len:SZ.t)
+  (credential_identity:array U8.t)
+  (credential_identity_len:SZ.t)
+  requires pts_to certificate_chain 'certificate_chain_bytes **
+           pts_to credential_identity 'credential_identity_bytes **
+           pure (B.length 'certificate_chain_bytes == SZ.v certificate_chain_len /\
+                 B.length 'credential_identity_bytes == SZ.v credential_identity_len)
+  returns s:server
+  ensures pts_to certificate_chain 'certificate_chain_bytes **
+          pts_to credential_identity 'credential_identity_bytes **
+          connection_exactly
+            s
+            (CR.server_initial_state
+              (Ghost.reveal 'certificate_chain_bytes)
+              (Ghost.reveal 'credential_identity_bytes)) **
+          pure (ST.server_state_correct
+                  (CR.server_initial_state
+                    (Ghost.reveal 'certificate_chain_bytes)
+                    (Ghost.reveal 'credential_identity_bytes)) /\
+                ST.server_end_to_end_invariant
+                  (CR.server_initial_state
+                    (Ghost.reveal 'certificate_chain_bytes)
+                    (Ghost.reveal 'credential_identity_bytes)) /\
+                CS.connection_state_raw_to_message_replay_consistent
+                  (CR.server_initial_state
+                    (Ghost.reveal 'certificate_chain_bytes)
+                    (Ghost.reveal 'credential_identity_bytes)) /\
+                CS.connection_state_sent_seal_replay_consistent
+                  (CR.server_initial_state
+                    (Ghost.reveal 'certificate_chain_bytes)
+                    (Ghost.reveal 'credential_identity_bytes)) /\
+                CS.connection_state_sent_seal_key_schedule_replay_consistent
+                  (CR.server_initial_state
+                    (Ghost.reveal 'certificate_chain_bytes)
+                    (Ghost.reveal 'credential_identity_bytes)) /\
+                CS.connection_state_received_decode_replay_consistent
+                  (CR.server_initial_state
+                    (Ghost.reveal 'certificate_chain_bytes)
+                    (Ghost.reveal 'credential_identity_bytes)) /\
+                CS.connection_state_received_decode_key_schedule_replay_consistent
+                  (CR.server_initial_state
+                    (Ghost.reveal 'certificate_chain_bytes)
+                    (Ghost.reveal 'credential_identity_bytes)) /\
+                CS.connection_state_protected_raw_segmented_replay_consistent
+                  (CR.server_initial_state
+                    (Ghost.reveal 'certificate_chain_bytes)
+                    (Ghost.reveal 'credential_identity_bytes)))
+{
+  let s =
+    CR.new_server
+      certificate_chain
+      certificate_chain_len
+      credential_identity
+      credential_identity_len;
+  ST.lemma_initial_server_state_correct
+    (CR.server_connection_config
+      (Ghost.reveal 'certificate_chain_bytes)
+      (Ghost.reveal 'credential_identity_bytes));
+  ST.lemma_initial_server_end_to_end_invariant
+    (CR.server_connection_config
+      (Ghost.reveal 'certificate_chain_bytes)
+      (Ghost.reveal 'credential_identity_bytes));
+  CSL.lemma_initial_raw_to_message_replay_consistent
+    (CR.server_connection_config
+      (Ghost.reveal 'certificate_chain_bytes)
+      (Ghost.reveal 'credential_identity_bytes));
+  CSL.lemma_initial_sent_seal_replay_consistent
+    (CR.server_connection_config
+      (Ghost.reveal 'certificate_chain_bytes)
+      (Ghost.reveal 'credential_identity_bytes));
+  CSL.lemma_initial_sent_seal_key_schedule_replay_consistent
+    (CR.server_connection_config
+      (Ghost.reveal 'certificate_chain_bytes)
+      (Ghost.reveal 'credential_identity_bytes));
+  CSL.lemma_initial_received_decode_replay_consistent
+    (CR.server_connection_config
+      (Ghost.reveal 'certificate_chain_bytes)
+      (Ghost.reveal 'credential_identity_bytes));
+  CSL.lemma_initial_received_decode_key_schedule_replay_consistent
+    (CR.server_connection_config
+      (Ghost.reveal 'certificate_chain_bytes)
+      (Ghost.reveal 'credential_identity_bytes));
+  ST.lemma_server_state_correct_protected_raw_segmented_replay
+    (CR.server_initial_state
+      (Ghost.reveal 'certificate_chain_bytes)
+      (Ghost.reveal 'credential_identity_bytes));
+  fold (connection_exactly
+    s
+    (CR.server_initial_state
+      (Ghost.reveal 'certificate_chain_bytes)
+      (Ghost.reveal 'credential_identity_bytes)));
+  s
+}
